\documentclass[12pt]{amsart}
\usepackage[margin=1in]{geometry}
\usepackage{ amssymb }

\newcommand{\Z}{\mathbb{Z}}
\newcommand{\N}{\mathbb{N}}
\newcommand{\R}{\mathbb{R}}
\renewcommand{\complement}{^{\mathsf{c}}}

\newtheorem*{proposition}{Proposition}

\title{301 Homework 36}
\author{Mark Kim}
\date{\today}

\begin{document}
\maketitle

\begin{proposition}
Let $x\in\R_{\geq 0}$ and $k\in\Z_{\geq 0}$.  Then
\begin{align*}
(1+x)^k \geq 1+kx.
\end{align*}
\end{proposition}

\begin{proof}
Let $x\in\R_{\geq 0}$ and $k\in\Z_{\geq 0}$, and proceed by induction on $k$.

For our base case, $k=0$,
\begin{align*}
(1+x)^0 &\geq 1 + 0\cdot x\\
1&\geq 1,
\end{align*}
which is certainly true.

Proceeding to the induction step, let us assume that for some $p\in\Z_{>0}$, $(1+x)^p \geq 1 +px$.  We need to show that
\begin{align*}
(1+x)^{p+1} \geq 1 + (p+1)x.
\end{align*}
Notice that
\begin{align*}
(1+x)^{p+1} = (1+x)^p (1+x) &\geq (1+px)(1+x)\\
&\geq 1+px+x+px^2\\
&\geq 1+(p+1)x +px^2.
\end{align*}
Since $p$ is positive and $x^2$ is always positive, we can can state
\begin{align*}
(1+x)^{p+1} &\geq 1+(p+1)x +px^2 \geq 1 + (p+1)x,
\end{align*}
proving our proposition.
\end{proof}
\end{document}